Finish channels

channel.v
@@ -29,6 +29,13 @@ Fixpoint append_l_s {A} (l : list A) (s : Stream A) :=
   | a :: l' => {|Shead := a; Stail := append_l_s l' s |}
   end.
 
+Lemma append_l_s_app {A} (vs : list A) v μ :
+  append_l_s (vs ++ [v]) μ = append_l_s vs {| Shead := v; Stail := μ |}.
+Proof.
+  induction vs; simpl; first done.
+  by rewrite IHvs.
+Qed.
+
 Class ChannelIG Σ := channelIG {
    stream_inG :> inG Σ (prodR (fracR) (agreeR (leibnizC (Stream val))));
    streams_inG :> inG Σ (prodR (fracR) (agreeR (leibnizC ((Stream val) → Prop))))
@@ -40,6 +47,15 @@ Fixpoint of_list (l : list val) :=
   | v :: l' => InjRV (PairV v (of_list l'))
   end.
 
+Global Instance of_list_inj : Inj eq eq of_list.
+Proof.
+  intros x.
+  induction x => y Heq; first by destruct y.
+  destruct y; first done.
+  inversion Heq; subst.
+  f_equal. by apply IHx.
+Qed.
+
 Section channels.
 
   Context `{!ChannelIG Σ, !heapIG Σ}.
@@ -50,23 +66,26 @@ Section channels.
   Definition own_streams γ q M :=
     own γ (q, to_agree M : (agreeR (leibnizC ((Stream val) → Prop)))).
 
-  Definition channel_inv queue γs1 γs2 γR : iProp Σ :=
-        (∃ vs (μ1 μ2 : Stream val) M,
+  Definition channel_inv chan γs1 γs2 γR : iProp Σ :=
+        (∃ vs (μ1 μ2 : Stream val) M queue l,
+            ⌜chan = (PairV (PrV l) (LocV queue))⌝ ∗
             queue ↦ (of_list vs) ∗
-                  own_stream γs1 (1/2)%Qp μ1 ∗
-                  own_stream γs2 (1/2)%Qp μ2 ∗
-                  own_streams γR (1/2)%Qp M ∗
-                  ⌜∀ μ', interleaving μ1 μ2 μ' → M (append_l_s vs μ')⌝
+            own_stream γs1 (1/2)%Qp μ1 ∗
+            own_stream γs2 (1/2)%Qp μ2 ∗
+            own_streams γR (1/2)%Qp M ∗
+            ⌜∀ μ', interleaving μ1 μ2 μ' → M (append_l_s vs μ')⌝
         )%I.
 
-  Definition sender queue μ :=
+  Definition sender chan μ :=
     (∃ γs γs1 γs2 γR,
-        inv (nroot .@ "channel") (channel_inv queue γs1 γs2 γR) ∗
+        inv (nroot .@ "channel") (channel_inv chan γs1 γs2 γR) ∗
             own_stream γs (1/2)%Qp μ ∗ ⌜γs = γs1 ∨ γs = γs2⌝)%I.
 
-  Definition receiver queue l μ :=
-    (∃ γs1 γs2 γR M, inv (nroot .@ "channel") (channel_inv queue γs1 γs2 γR)
-                         ∗ own_streams γR (1/2)%Qp M ∗ cpvar l M μ)%I.
+  Definition receiver chan μ :=
+    (∃ γs1 γs2 γR M queue l,
+        ⌜chan = (PairV (PrV l) (LocV queue))⌝ ∗
+        inv (nroot .@ "channel") (channel_inv chan γs1 γs2 γR)
+            ∗ own_streams γR (1/2)%Qp M ∗ cpvar l M μ)%I.
 
   Definition new_channel :=
     Lam (Pair Create_Pr (Alloc (InjL Plang.Unit))).
@@ -74,9 +93,9 @@ Section channels.
   Lemma wp_new_channel μ1 μ2 :
     {{{True}}}
       App new_channel Plang.Unit
-    {{{q l, RET (PairV (PrV l) (LocV q));
-       sender q μ1 ∗ sender q μ2 ∗
-              ∃ μ, ⌜interleaving μ1 μ2 μ⌝ ∗ receiver q l μ
+    {{{w, RET w;
+       sender w μ1 ∗ sender w μ2 ∗
+              ∃ μ, ⌜interleaving μ1 μ2 μ⌝ ∗ receiver w μ
     }}}.
   Proof.
     iIntros (Φ) "_ HΦ".
@@ -100,70 +119,315 @@ Section channels.
                      : (agreeR (leibnizC (Stream val → Prop)))))
       as (γR) "[HM1 HM2]";
       first done.
-    iMod (inv_alloc (nroot .@ "channel") _ (channel_inv q γs1 γs2 γR)
+    iMod (inv_alloc (nroot .@ "channel") _
+                    (channel_inv (PairV (PrV l) (LocV q)) γs1 γs2 γR)
             with "[Hμ11 Hμ21 HM1 Hq]") as "#Hinv".
     { iNext. unfold channel_inv.
-      iExists [], _, _, _; iFrame; auto. }
+      iExists [], _, _, _, _, _; iFrame; eauto. }
     iModIntro.
     iApply "HΦ".
     iSplitL "Hμ12"; first by iExists _, _, _, _; iFrame; iFrame "#"; eauto.
     iSplitL "Hμ22"; first by iExists _, _, _, _; iFrame; iFrame "#"; eauto.
     iExists μ; iSplit; first by iApply cpvar_contains.
-    iExists _, _, _, _; iFrame "#"; iFrame.
+    iExists _, _, _, _, _, _; iFrame "#"; iFrame; eauto.
   Qed.
 
-  Definition Append :=
-    Lam
-      (Rec
+  Definition append :=
+    Rec
+      (Lam
          (Case
-            (Var 1) (Var 3)
-            (InjR (Pair (Fst (Var 0)) (App (Var 1) (Snd (Var 0)))) ))
+            (Var 2) (Var 1)
+            (InjR
+               (Pair (Fst (Var 0)) (App (App (Var 2) (Snd (Var 0))) (Var 1)))
+            )
+         )
       ).
+  Lemma append_eq :
+    append = Rec
+      (Lam
+         (Case
+            (Var 2) (Var 1)
+            (InjR
+               (Pair (Fst (Var 0)) (App (App (Var 2) (Snd (Var 0))) (Var 1)))
+            )
+         )
+      ).
+  Proof. trivial. Qed.
 
-  Lemma wp_Append `{heapIG Σ} l l' :
-    WP (App (App Append (of_val (of_list l))) (of_val (of_list l')))
-       {{w, ⌜w = of_list (l' ++ l)⌝}}%I.
+  Typeclasses Opaque append.
+  Global Opaque append.
+
+  Lemma wp_append `{heapIG Σ} l l' :
+    {{{True}}} (App (App append (of_val (of_list l))) (of_val (of_list l')))
+       {{{w, RET w; ⌜w = of_list (l ++ l')⌝}}}.
   Proof.
+    iIntros (Φ) "_ HΦ".
+    iLöb as "IH" forall (Φ l).
+    rewrite append_eq.
     iApply (wp_bind (fill [AppLCtx _])).
     iApply wp_pure_step_later; auto.
-    iNext.
-    asimpl.
+    rewrite -append_eq.
+    iNext. asimpl.
     iApply wp_value. simpl.
-    iLöb as "IH" forall (l').
-                   iApply wp_pure_step_later; auto.
-                   iNext.
-                   asimpl.
-                   destruct l'.
-                   - simpl. iApply wp_pure_step_later; auto.
-                     iNext. asimpl. by iApply wp_value.
-                   - simpl. iApply wp_pure_step_later; auto.
-                     iNext. asimpl.
-                     iApply (wp_bind (fill [InjRCtx])).
-                     iApply (wp_bind (fill [PairLCtx _])).
-                     iApply wp_pure_step_later; auto.
-                     iNext; iApply wp_value. simpl.
-                     iApply (wp_bind (fill [PairRCtx _])).
-                     iApply (wp_bind (fill [AppRCtx (RecV _)])).
-                     iApply wp_pure_step_later; auto.
-                     iNext; iApply wp_value. simpl.
-                     iApply wp_wand_r; iSplitR.
-                     { iApply "IH". }
-                     iIntros (w) "%"; subst; simpl.
-                       by do 2 iApply wp_value.
+    iApply wp_pure_step_later; auto.
+    iNext. asimpl.
+    destruct l.
+    - simpl. iApply wp_pure_step_later; eauto.
+      iNext. asimpl. iApply wp_value. by iApply "HΦ".
+    - simpl. iApply wp_pure_step_later; auto.
+      iNext. asimpl.
+      iApply (wp_bind (fill [InjRCtx])).
+      iApply (wp_bind (fill [PairLCtx _])).
+      iApply wp_pure_step_later; auto.
+      iNext; iApply wp_value. simpl.
+      iApply (wp_bind (fill [PairRCtx _])).
+      rewrite append_eq.
+      iApply (wp_bind (fill [AppRCtx (RecV _); AppLCtx _])).
+      rewrite /= -append_eq.
+      iApply wp_pure_step_later; auto.
+      iNext; iApply wp_value.
+      iApply wp_wand_r; iSplitR.
+      { iApply ("IH" $! (λ s, ⌜s = of_list (l ++ l')⌝))%I. iNext.
+        by iIntros (w Hw); subst w. }
+      simpl.
+      iIntros (w) "%"; subst; simpl.
+      do 2 iApply wp_value.
+      by iApply "HΦ".
   Qed.
 
   Definition send :=
     Lam
       (Rec
-         (LetIn (Load (Snd (Var 2)))
-                (If
-                   (CAS (Snd (Var 3)) (Var 0) (App (App Append (Var 2)) (Var 3)))
-                   (Plang.Unit)
-                   (App (Var 1) (Var 2))
-                )
+         (LetIn
+            (Snd (Var 2))
+            (LetIn
+               (Load (Var 0))
+               (If
+                  (CAS (Var 1) (Var 0)
+                       (App (App append.[ren (+5)]
+                                          (Var 0))
+                            (InjR (Pair (Var 3) (InjL Unit)))))
+                  Unit
+                  (App (Var 2) (Var 3))
+               )
+            )
          )
       ).
 
+  Lemma wp_send chan v μ :
+    {{{sender chan {| Shead := v; Stail := μ|} }}}
+      App (App send (of_val chan)) (of_val v)
+      {{{RET UnitV;  sender chan μ }}}.
+  Proof.
+    iIntros (Φ) "HP HΦ".
+    iDestruct "HP" as (γs γs1 γs2 γR) "(#chinv & Hγs & #Hγseq)".
+    iApply fupd_wp.
+    iInv (nroot.@"channel") as "Hinv" "Hcl".
+    iDestruct "Hinv" as (ws μ1 μ2 M queue l) "(>% & ? & ? & ? & ? & ?)";
+      simplify_eq.
+    iMod ("Hcl" with "[- Hγs HΦ]") as "_";
+      first by iExists _, _, _, _, _, _; iNext; iFrame.
+    iModIntro.
+    clear ws μ1 μ2 M.
+    iApply (wp_bind (fill [AppLCtx _])).
+    iApply wp_pure_step_later; trivial.
+    iNext. asimpl.
+    iApply wp_value; simpl.
+    iLöb as "IH".
+    iApply wp_pure_step_later; trivial.
+    iNext. asimpl.
+    iApply (wp_bind (fill [LetInCtx _])).
+    iApply wp_pure_step_later; trivial.
+    iNext; iApply wp_value; simpl.
+    iApply wp_pure_step_later; trivial.
+    iNext; asimpl.
+    iApply (wp_bind (fill [LetInCtx _])).
+    iInv (nroot.@"channel") as "Hinv" "Hcl".
+    iDestruct "Hinv" as (ws μ1 μ2 M queue' l') "(>% & Hq & ? & ? & ? & ?)";
+      simplify_eq.
+    iApply (wp_load with "Hq"); first iFrame.
+    iNext. iIntros "Hq".
+    iMod ("Hcl" with "[- Hγs HΦ]") as "_";
+      first by iExists _, _, _, _, _, _; iNext; iFrame.
+    clear μ1 μ2 M.
+    iModIntro.
+    iApply wp_pure_step_later; trivial.
+    iNext. asimpl.
+    iApply (wp_bind (fill [IfCtx _ _])).
+    iApply (wp_bind (fill [CasRCtx (LocV _) _])); simpl.
+    iApply (wp_append _ [v]); trivial.
+    iNext; simpl.
+    iIntros (w ?); subst w.
+    iInv (nroot.@"channel") as "Hinv" "Hcl".
+    iDestruct "Hinv" as (ws' μ1 μ2 M queue l)
+                          "(>% & Hq & Hγs1 & Hγs2 & HγR & >Hintr)"; simplify_eq.
+    iDestruct "Hintr" as %Hintr.
+    destruct (decide (ws' = ws)) as [|Hneq]; first subst ws'.
+    - iApply (wp_cas_suc with "Hq").
+      iNext. iIntros "Hq".
+      iAssert (|={⊤ ∖ ↑nroot.@"channel",⊤}=>
+              own_stream γs (1 / 2)%Qp μ)%I with "[-HΦ]" as "Hcl".
+      { iDestruct "Hγseq" as %[]; subst γs.
+        - iDestruct (own_valid_2 with "Hγs Hγs1") as %[_ ?%agree_op_invL'];
+          simpl in *; simplify_eq.
+          iCombine "Hγs" "Hγs1" as "Hγs".
+          iMod (own_update _ _ ((1%Qp, to_agree μ : agreeR (leibnizC _)))
+                  with "Hγs") as "[Hγs Hγys1]".
+          { by apply cmra_update_exclusive. }
+          iMod ("Hcl" with "[- Hγs]") as "_"; last by iFrame.
+          { iExists _, _, _, _, _, _; iNext; iFrame.
+            iSplit; first by eauto.
+            iPureIntro. intros; rewrite append_l_s_app.
+            apply Hintr; by econstructor. }
+        - iDestruct (own_valid_2 with "Hγs Hγs2") as %[_ ?%agree_op_invL'];
+          simpl in *; simplify_eq.
+          iCombine "Hγs" "Hγs2" as "Hγs".
+          iMod (own_update _ _ ((1%Qp, to_agree μ : agreeR (leibnizC _)))
+                  with "Hγs") as "[Hγs Hγs2]".
+          { by apply cmra_update_exclusive. }
+          iMod ("Hcl" with "[- Hγs]") as "_"; last by iFrame.
+          { iExists _, _, _, _, _, _; iNext; iFrame.
+            iSplit; first by eauto.
+            iPureIntro. intros; rewrite append_l_s_app.
+            apply Hintr; by econstructor. }
+      }
+      iMod "Hcl" as "Hγs".
+      iModIntro.
+      iApply wp_pure_step_later; trivial.
+      iNext. asimpl.
+      iApply wp_value.
+      iApply "HΦ".
+      iExists _, _, _, _; iFrame "#"; iFrame.
+    - iApply (wp_cas_fail with "Hq").
+      { intros ?; apply Hneq; eapply (@inj _ _ eq eq of_list _); eauto. }
+      iNext. iIntros "Hq".
+      iMod ("Hcl" with "[- Hγs HΦ]") as "_";
+      first by iExists _, _, _, _, _, _; iNext; iFrame.
+      iModIntro.
+      iApply wp_pure_step_later; trivial.
+      iNext. by iApply ("IH" with "Hγs").
+  Qed.
+
+  Definition receive :=
+    Lam
+      (LetIn
+         (Fst (Var 0))
+         (LetIn
+            (Snd (Var 1))
+            (App
+               (Rec
+                  (LetIn
+                     (Load (Var 2))
+                     (Case
+                        (Var 0)
+                        (App (Var 2) Unit)
+                        (If
+                           (CAS (Var 4) (Var 1) (Snd (Var 0)))
+                           (LetIn
+                              (Fst (Var 0))
+                              (Seq
+                                 (Assign_Pr (Var 6) (Var 0))
+                                 (Var 0)
+                              )
+                           )
+                           (App (Var 2) Unit)
+                        )
+                     )
+                  )
+               )
+               Unit
+            )
+         )
+      ).
+
+  Lemma wp_receive chan v μ :
+    {{{receiver chan {| Shead := v; Stail := μ|} }}}
+      App receive (of_val chan)
+      {{{RET v;  receiver chan μ }}}.
+  Proof.
+    iIntros (Φ) "HP HΦ".
+    iDestruct "HP" as (γs1 γs2 γR M q l Hcn) "(#chinv & HR & Hpr)"; subst.
+    iApply wp_pure_step_later; trivial.
+    iNext. asimpl.
+    iApply (wp_bind (fill [LetInCtx _])).
+    iApply wp_pure_step_later; trivial.
+    iNext; iApply wp_value; simpl.
+    iApply wp_pure_step_later; trivial.
+    iNext. asimpl.
+    iApply (wp_bind (fill [LetInCtx _])).
+    iApply wp_pure_step_later; trivial.
+    iNext; iApply wp_value; simpl.
+    iApply wp_pure_step_later; trivial.
+    iNext. asimpl.
+    iLöb as "IH".
+    iApply wp_pure_step_later; trivial.
+    iNext. asimpl.
+    iApply (wp_bind (fill [LetInCtx _])).
+    iInv (nroot.@"channel") as "Hinv" "Hcl".
+    iDestruct "Hinv" as (ws μ1 μ2 M' queue' l') "(>% & Hq & ? & ? & ? & ?)";
+      simplify_eq.
+    iApply (wp_load with "Hq"); first iFrame.
+    iNext. iIntros "Hq".
+    iMod ("Hcl" with "[- HR Hpr HΦ]") as "_";
+      first by iExists _, _, _, _, _, _; iNext; iFrame.
+    clear μ1 μ2 M'.
+    iModIntro.
+    iApply wp_pure_step_later; trivial.
+    iNext. asimpl.
+    destruct ws as [|w ws]; simpl.
+    { iApply wp_pure_step_later; trivial.
+      iNext. asimpl.
+      by iApply ("IH" with "HR Hpr"). }
+    iApply wp_pure_step_later; trivial.
+    iNext. asimpl.
+    iApply (wp_bind (fill [IfCtx _ _])).
+    iApply (wp_bind (fill [CasRCtx (LocV _) (InjRV (PairV _ _))])); simpl.
+    iApply wp_pure_step_later; trivial.
+    iNext; iApply wp_value; simpl.
+    iInv (nroot.@"channel") as "Hinv" "Hcl".
+    iDestruct "Hinv" as (ws' μ1 μ2 M' queue l)
+                          "(>% & Hq & Hγs1 & Hγs2 & HγR & >Hintr)"; simplify_eq.
+    iDestruct "Hintr" as %Hintr.
+    destruct (decide (ws' = w :: ws)) as [|Hneq]; first subst ws'.
+    - iApply (wp_cas_suc with "Hq").
+      iNext. iIntros "Hq".
+      iDestruct (own_valid_2 with "HR HγR") as %[_ ?%agree_op_invL'];
+        simpl in *; simplify_eq.
+      iCombine "HR" "HγR" as "HR".
+      iMod (own_update
+              _ _
+              ((1%Qp, to_agree (λ μ, M' {| Shead := w; Stail := μ |})
+                : agreeR (leibnizC _)))
+              with "HR") as "[HR HγR]".
+      { by apply cmra_update_exclusive. }
+      iMod ("Hcl" with "[- HR Hpr HΦ]") as "_".
+      { iExists _, _, _, _, _, _; iNext; iFrame; eauto. }
+      iModIntro.
+      iApply wp_pure_step_later; trivial.
+      iNext.
+      iApply (wp_bind (fill [LetInCtx _])).
+      iApply wp_pure_step_later; trivial.
+      iNext; iApply wp_value; simpl.
+      iApply wp_pure_step_later; trivial.
+      iNext. asimpl.
+      iApply (wp_bind (fill [SeqCtx _])).
+      iApply (wp_assign_pr with "[$Hpr]").
+      { iExists (append_l_s ws _); iPureIntro.
+        eapply Hintr, interleaving_inh. }
+      iNext. iIntros "[% Hpr]"; subst; simpl.
+      iApply wp_pure_step_later; trivial.
+      iNext; iApply wp_value.
+      iApply "HΦ".
+      iExists _, _, _, _, _, _; iFrame "#"; iFrame; eauto.
+    - iApply (wp_cas_fail with "Hq").
+      { intros ?; apply Hneq; eapply (@inj _ _ eq eq of_list _); eauto. }
+      iNext. iIntros "Hq".
+      iMod ("Hcl" with "[- HR Hpr HΦ]") as "_";
+      first by iExists _, _, _, _, _, _; iNext; iFrame.
+      iModIntro.
+      iApply wp_pure_step_later; trivial.
+      iNext. by iApply ("IH" with "HR Hpr").
+  Qed.
 
 End channels.
 
